theories/ordinals/solutions_exercises/OnCodeList.v
@@ -1,0 +1,34 @@
+(* begin snippet membersDef:: no-out *)
+Require Import primRec cPair Arith.
+From Equations Require Import  Equations.
+
+Equations members (a:nat): list nat by wf a:=
+  members 0 := List.nil;
+  members (S z) := cPairPi1 z:: members (cPairPi2 z).
+(* end snippet membersDef *)
+Next Obligation.
+  apply Nat.le_lt_trans with z.
+  apply cPairLe2A.
+  apply le_n.
+Defined.
+
+Lemma membersOk n : n = codeList (members n).
+Proof.
+     pattern n, (members n); apply members_elim. 
+      -  reflexivity. 
+      -  intros; simpl; f_equal; rewrite <- H. 
+         now rewrite cPairProjections.
+Qed. 
+
+Lemma membersOk' l : l = members (codeList l).
+Proof.
+  induction l. 
+  - reflexivity.
+   - cbn; rewrite IHl. 
+     rewrite members_equation_2. 
+     now rewrite cPairProjections1, cPairProjections2, <- !IHl.
+Qed. 
+
+
+
+  
